FPVFinalSAT.lean
@@ -1,2 +1,5 @@
 import FPVFinalSAT.TwoSAT
+import FPVFinalSAT.Graphs
 import FPVFinalSAT.ImplicationGraph
+import FPVFinalSAT.Semantics
+import FPVFinalSAT.Correctness
